updates

Veritas.Verifier.EAC.fst
@@ -35,24 +35,24 @@ type hash_collision_gen =
   | MultiHashCollision: hc: ms_hash_collision -> hash_collision_gen
 
 (* construct a hash collision from a contradiction *)
-let hash_collision_contra (_:unit{False}): hash_collision_gen = 
+let hash_collision_contra (_:unit{False}): hash_collision_gen =
   SingleHashCollision (Collision (DVal Null) (DVal Null))
 
 (* if an operation requires the key in store, it cannot be the first operation *)
-let lemma_non_eac_init_requires_key_in_store 
+let lemma_non_eac_init_requires_key_in_store
   (itsl: neac_log {
     eac_boundary_state_pre itsl = EACInit /\
     requires_key_in_store (eac_boundary_entry itsl) /\
     Root <> key_of (eac_boundary_entry itsl)
-  }): 
-  hash_collision_gen =   
+  }):
+  hash_collision_gen =
   // maximum prefix of itsl that is eac
-  let i = eac_boundary itsl in  
+  let i = eac_boundary itsl in
   let itsli = I.prefix itsl i in
 
-  // vlog entry e going at thread tid causes the eac failure 
+  // vlog entry e going at thread tid causes the eac failure
   let e = I.index itsl i in
-  let k = V.key_of e in  
+  let k = V.key_of e in
   let tid = thread_id_of itsl i in
 
   // Store of tid does not contain the key k after processing i elements
@@ -61,16 +61,14 @@ let lemma_non_eac_init_requires_key_in_store
 
   // but we know that the tid state is still valid after processing e
   // which does require k to be in the store, a contradiction
-  TL.lemma_verifier_thread_state_extend itsl i;
-  
   hash_collision_contra ()
 
 (* the first operation for a key cannot be evict *)
-let lemma_non_eac_init_evict 
+let lemma_non_eac_init_evict
   (itsl: neac_log {
     eac_boundary_state_pre itsl = EACInit /\
     V.is_evict (eac_boundary_entry itsl)
-  }): hash_collision_gen =  
+  }): hash_collision_gen =
   let i = TL.eac_boundary itsl in
   TL.lemma_root_never_evicted itsl i;
   lemma_non_eac_init_requires_key_in_store itsl
@@ -80,137 +78,118 @@ let lemma_non_eac_init_addb
   (itsl: neac_log {
     TL.hash_verifiable itsl /\
     eac_boundary_state_pre itsl = EACInit /\
-    AddB? (eac_boundary_entry itsl)}): hash_collision_gen =
-  admit()
-  (*
-  (* hash verifiable - evict hash and add hash equal *)                          
-  let gl = partition_idx_seq itsl in                           
-  assert(VG.hadd gl = VG.hevict gl);
+    is_blum_add (eac_boundary_entry itsl)}): hash_collision_gen =
 
-  let tsle = time_seq_ext itsl in
-  let i = max_eac_prefix tsle in
-  let (e,tid) = index itsl i in
-  let k = V.key_of e in
+  (* the maximum eac prefix of itsl *)
+  let i = eac_boundary itsl in
+  let itsli = I.prefix itsl i in
 
-  (* the i'th entry is a blum add *)
-  assert(is_blum_add (index itsl i));
-  let be = blum_add_elem (index itsl i) in
-  
-  (* pre-condition: state of key after processing i entries i EACInit *)
-  let itsli = prefix itsl i in
-  assert(eac_state_of_key itsli k = EACInit);
+  let gl = g_vlog_of itsl in
 
-  (* the first i entries cannot contain any entry with key k *)
-  lemma_eac_init_implies_no_key_entries itsli k;
-  assert(not (has_some_entry_of_key itsli k));
+  // the blum add element corresponding to the boundary
+  let e = I.index itsl i in
+  let k = key_of e in
+  let be = blum_add_elem (I.index itsl i) in
 
-  (* if the add element be is in the evict set *)
+  // since k is in init_state after processing i entries, there cannot
+  // be a prior entry for k
+  lemma_eac_state_init_no_entry itsli k;
+  //assert(not (has_some_entry_of_key itsli k));
+
   if MS.contains be (ts_evict_set itsl) then (
     (* the evict that corresponds to blum add happens before i *)
     let j = index_blum_evict itsl be in
     lemma_evict_before_add itsl i;
-    assert(j < i);
+    //assert(j < i);
 
     (* this emplies itsli contains an entry with key k *)
     (* a contradiction *)
-    lemma_last_index_correct2 (entry_of_key k) itsli j;
-    
-    hash_collision_contra ()                           
+    assert(index (I.i_seq itsli) j = I.index itsli j);
+    lemma_last_index_correct2 (is_entry_of_key k) (I.i_seq itsli) j;
+    hash_collision_contra ()
   )
-  else (  
+  else (
+    (* since be is in add set, but not in evict set they cannot be the same *)
     lemma_add_elem_correct itsl i;
     lemma_ts_add_set_correct itsl;
     lemma_ts_evict_set_correct itsl;
-
-    assert(MS.contains be (ts_add_set itsl));
-    assert(not (MS.contains be (ts_evict_set itsl)));
-    
-    lemma_ts_add_set_correct itsl;
-    lemma_ts_evict_set_correct itsl;
-
-    assert(ts_add_set itsl == g_add_set gl);
-    assert(ts_evict_set itsl == g_evict_set gl);
-    MS.lemma_not_equal (g_add_set gl) (g_evict_set gl) be;    
-    assert(~ (g_add_set gl == g_evict_set gl));
+    MS.lemma_not_equal (g_add_set gl) (g_evict_set gl) be;
+    //assert(~ (g_add_set gl == g_evict_set gl));
 
     lemma_g_hadd_correct gl;
     lemma_ghevict_correct gl;
 
     MultiHashCollision (MSCollision (g_add_seq gl) (g_evict_seq gl))
   )
-*)
-
-(*
-
 
 let lemma_non_eac_init_addm
-  (#p:pos) 
-  (itsl: non_eac_ts_log p{
-    last_valid_eac_state itsl = EACInit /\
-    AddM? (to_vlog_entry (invalidating_log_entry itsl))
+  (itsl: neac_log{
+    eac_boundary_state_pre itsl = EACInit /\
+    is_merkle_add (eac_boundary_entry itsl)
    })
-   : hash_collision_gen =
-   
-  let st = last_valid_eac_state itsl in   
-  let ee = invalidating_log_entry itsl in
-  assert(eac_add ee st = EACFail);
+  : hash_collision_gen =
+  (* the maximum eac prefix of itsl *)
+  let i = eac_boundary itsl in
+  let itsli = I.prefix itsl i in
+  let itsli' = I.prefix itsl (i + 1) in
 
-  let tsle = time_seq_ext itsl in
-  let i = max_eac_prefix tsle in
-  let (e,tid) = index itsl i in
-  assert(to_vlog_entry ee = e);
+  // vlog entry e going at thread tid causes the eac failure
+  let e = I.index itsl i in
+  let k = V.key_of e in
+  let tid = thread_id_of itsl i in
+  let ee = TL.vlog_entry_ext_at itsl i in
 
-  let itsli = prefix itsl i in
-  let vsi = verifier_thread_state itsli tid in
-  let itsli' = prefix itsl (i+1) in
-  let vsi' = verifier_thread_state itsli' tid in
-  
-  lemma_verifier_thread_state_extend itsli';  
-  assert(vsi' == t_verify_step vsi e);
+  //assert(eac_add ee (eac_boundary_state_pre itsl) = EACFail);                 
   match e with
-  | AddM (k,v) k' -> 
-    (* otherwise eac_add ee st <> EACFail *)
-    assert(v <> init_value k);
+  | AddM (k,v) k' ->
+    
+    (* otherwise eac_add ee (boundary_state ...) <> EACFail *)
+    // assert(v <> init_value k);
 
     (* verifier checks this *)
-    assert(is_proper_desc k k');
+    // assert(is_proper_desc k k');
 
     (* k' is the proving ancestor of k*)
     lemma_addm_ancestor_is_proving itsli';
-    assert(k' = proving_ancestor itsli k);
+    //assert(k' = proving_ancestor itsli k);
 
     (* k' is the verifier cache *)
-    assert(store_contains (thread_store vsi) k');
+    //assert(store_contains (thread_store itsli tid) k');
+
     lemma_eac_value_is_stored_value itsli k' tid;
-    assert(eac_value itsli k' = stored_value (thread_store vsi) k');
+    //assert(eac_value itsli k' = V.stored_value (thread_store itsli tid) k');
 
     let v' = eac_merkle_value itsli k' in
-    assert(v' = to_merkle_value( stored_value (thread_store vsi) k'));
+    //assert(v' = to_merkle_value(V.stored_value (thread_store itsli tid) k'));
+
     let d = desc_dir k k' in
     let dh' = desc_hash_dir v' d in
 
     (* k' points to none or some non-ancestor of k *)
-    assert(is_eac_state_init itsli k);
+    //assert(is_eac_state_init itsli k);
     lemma_proving_ancestor_initial itsli k;
-
-    assert(mv_points_to_none v' d \/ 
-          not (is_desc k (mv_pointed_key v' d)));
+    //assert(mv_points_to_none v' d \/ not (is_desc k (mv_pointed_key v' d)));
 
     match dh' with
     | Empty -> hash_collision_contra()
-    | Desc k2 _ _ -> 
-      assert(not (is_desc k k2));
+    | Desc k2 _ _ ->
+      //assert(not (is_desc k k2));
       lemma_desc_reflexive k;
-      assert(k <> k2);
+      //assert(k <> k2);
       hash_collision_contra()
 
-let lemma_non_eac_instore_get (#p:pos)   
+
+(*
+
+
+
+let lemma_non_eac_instore_get (#p:pos)
   (itsl: non_eac_ts_log p{
     EACInStore? (last_valid_eac_state itsl)  /\
     Get? (to_vlog_entry (invalidating_log_entry itsl))
    })
-  : hash_collision_gen = 
-  let st = last_valid_eac_state itsl in   
+  : hash_collision_gen =
+  let st = last_valid_eac_state itsl in
   let ee = invalidating_log_entry itsl in
   assert(eac_add ee st = EACFail);
 
@@ -223,14 +202,14 @@ let lemma_non_eac_instore_get (#p:pos)
   let vsi = verifier_thread_state itsli tid in
   let itsli' = prefix itsl (i+1) in
   let vsi' = verifier_thread_state itsli' tid in
-  
-  lemma_verifier_thread_state_extend itsli';  
+
+  lemma_verifier_thread_state_extend itsli';
   assert(vsi' == t_verify_step vsi e);
 
-  match st with 
+  match st with
   | EACInStore m v -> (
-    match ee with 
-    | NEvict (Get k v') -> 
+    match ee with
+    | NEvict (Get k v') ->
       (* otherwise there will not be an eac failure *)
       assert(DVal v' <> v);
 
@@ -248,7 +227,7 @@ let lemma_non_eac_instore_get (#p:pos)
         hash_collision_contra()
       )
       else (
-        (* if the get goes to tid <> tid_add, then the cache of tid does not contain k *)   
+        (* if the get goes to tid <> tid_add, then the cache of tid does not contain k *)
         lemma_eac_state_instore2 itsli k tid;
         assert(not (store_contains (thread_store vsi) k));
 
@@ -257,13 +236,13 @@ let lemma_non_eac_instore_get (#p:pos)
       )
   )
 
-let lemma_non_eac_instore_put (#p:pos)   
+let lemma_non_eac_instore_put (#p:pos)
   (itsl: non_eac_ts_log p{
     EACInStore? (last_valid_eac_state itsl)  /\
     Put? (to_vlog_entry (invalidating_log_entry itsl))
    })
-  : hash_collision_gen = 
-  let st = last_valid_eac_state itsl in   
+  : hash_collision_gen =
+  let st = last_valid_eac_state itsl in
   let ee = invalidating_log_entry itsl in
   assert(eac_add ee st = EACFail);
 
@@ -276,14 +255,14 @@ let lemma_non_eac_instore_put (#p:pos)
   let vsi = verifier_thread_state itsli tid in
   let itsli' = prefix itsl (i+1) in
   let vsi' = verifier_thread_state itsli' tid in
-  
-  lemma_verifier_thread_state_extend itsli';  
+
+  lemma_verifier_thread_state_extend itsli';
   assert(vsi' == t_verify_step vsi e);
 
-  match st with 
+  match st with
   | EACInStore m v -> (
-    match ee with 
-    | NEvict (Put k v') -> 
+    match ee with
+    | NEvict (Put k v') ->
       assert(not (DVal? v));
 
       (* the thread id where k was last added *)
@@ -299,18 +278,18 @@ let lemma_non_eac_instore_put (#p:pos)
       hash_collision_contra()
   )
 
-let lemma_non_eac_instore_addb (#p:pos)   
+let lemma_non_eac_instore_addb (#p:pos)
   (itsl: non_eac_ts_log p{
     VG.hash_verifiable (partition_idx_seq itsl) /\
     EACInStore? (last_valid_eac_state itsl)  /\
     AddB? (to_vlog_entry (invalidating_log_entry itsl))
    })
-  : hash_collision_gen = 
-  (* hash verifiable - evict hash and add hash equal *)                          
-  let gl = partition_idx_seq itsl in                           
+  : hash_collision_gen =
+  (* hash verifiable - evict hash and add hash equal *)
+  let gl = partition_idx_seq itsl in
   assert(VG.hadd gl = VG.hevict gl);
 
-  let st = last_valid_eac_state itsl in   
+  let st = last_valid_eac_state itsl in
   let ee = invalidating_log_entry itsl in
   assert(eac_add ee st = EACFail);
 
@@ -339,18 +318,18 @@ let lemma_non_eac_instore_addb (#p:pos)
   lemma_ts_evict_set_key_extend2 itsli';
   assert(ts_evict_set_key itsli' k == ts_evict_set_key itsli k);
 
-  (* this implies that the size of the add set after processing (i+1) elements 
+  (* this implies that the size of the add set after processing (i+1) elements
    * is one larger than the evict set at this point *)
   assert(MS.size (ts_add_set_key itsli' k) = 1 + (MS.size (ts_evict_set_key itsli' k)));
 
-  (* this implies that in the first (i+1) entries there is an element whose membership in 
+  (* this implies that in the first (i+1) entries there is an element whose membership in
    * add multiset is > its membership in evict multiset *)
-  let be = diff_elem (ts_add_set_key itsli' k) (ts_evict_set_key itsli' k) in  
+  let be = diff_elem (ts_add_set_key itsli' k) (ts_evict_set_key itsli' k) in
   assert(MS.contains be (ts_add_set_key itsli' k));
   lemma_ts_add_set_key_contains_only itsli' k be;
   assert(MH.key_of be = k);
   lemma_mem_key_add_set_same itsli' be;
-  lemma_mem_key_evict_set_same itsli' be;  
+  lemma_mem_key_evict_set_same itsli' be;
   assert(MS.mem be (ts_add_set itsli') > MS.mem be (ts_evict_set itsli'));
 
   (* the index of be in the add set *)
@@ -369,7 +348,7 @@ let lemma_non_eac_instore_addb (#p:pos)
 
   (* this implies the membership of be in (overall) addset > membership in evict set *)
   (* so these two sets are not equal providing a hash collision *)
-  assert(MS.mem be (ts_add_set itsl) > MS.mem be (ts_evict_set itsl));  
+  assert(MS.mem be (ts_add_set itsl) > MS.mem be (ts_evict_set itsl));
 
   MS.lemma_not_equal (ts_add_set itsl) (ts_evict_set itsl) be;
   assert(~( (ts_add_set itsl) == (ts_evict_set itsl)));
@@ -384,17 +363,17 @@ let lemma_non_eac_instore_addb (#p:pos)
 
   MultiHashCollision (MSCollision (g_add_seq gl) (g_evict_seq gl))
 
-let lemma_non_eac_instore_addm (#p:pos)   
+let lemma_non_eac_instore_addm (#p:pos)
   (itsl: non_eac_ts_log p{
     EACInStore? (last_valid_eac_state itsl)  /\
     AddM? (to_vlog_entry (invalidating_log_entry itsl))
    })
-  : hash_collision_gen = 
+  : hash_collision_gen =
   let tsle = time_seq_ext itsl in
-  let i = max_eac_prefix tsle in  
+  let i = max_eac_prefix tsle in
   let (e,tid) = index itsl i in
   let k = V.key_of e in
-  let itsli = prefix itsl i in    
+  let itsli = prefix itsl i in
 
   (* verifier thread state of tid after itsli *)
   let vsi = verifier_thread_state itsli tid in
@@ -404,13 +383,13 @@ let lemma_non_eac_instore_addm (#p:pos)
   let ltid = last_add_tid itsli k in
 
   let itsli' = prefix itsl (i + 1) in
-  let vsi' = verifier_thread_state itsli' tid in      
-  lemma_verifier_thread_state_extend itsli';    
-  assert(vsi' == t_verify_step vsi e);      
+  let vsi' = verifier_thread_state itsli' tid in
+  lemma_verifier_thread_state_extend itsli';
+  assert(vsi' == t_verify_step vsi e);
 
   if ltid = tid then (
     (* the store of tid contains the key k already *)
-    assert(store_contains (thread_store vsi) k);    
+    assert(store_contains (thread_store vsi) k);
 
     (* if store of tid already contained k then verifier should fail - a contradiction *)
     hash_collision_contra()
@@ -447,11 +426,11 @@ let lemma_non_eac_instore_addm (#p:pos)
       )
     )
     else (
-      
+
       lemma_instore_implies_eac_state_instore itsli k' ltid;
       assert(is_eac_state_instore itsli k');
-      
-      lemma_eac_state_instore itsli k';            
+
+      lemma_eac_state_instore itsli k';
 
       (* last add thread id of k' *)
       let ltid' = last_add_tid itsli k' in
@@ -470,20 +449,20 @@ let lemma_non_eac_instore_addm (#p:pos)
     )
   )
 
-let lemma_non_eac_instore_evictm (#p:pos)   
+let lemma_non_eac_instore_evictm (#p:pos)
   (itsl: non_eac_ts_log p{
     EACInStore? (last_valid_eac_state itsl)  /\
     EvictM? (to_vlog_entry (invalidating_log_entry itsl))
    })
-  : hash_collision_gen = 
-  let st = last_valid_eac_state itsl in   
+  : hash_collision_gen =
+  let st = last_valid_eac_state itsl in
   let ee = invalidating_log_entry itsl in
   assert(eac_add ee st = EACFail);
 
   match st with
   | EACInStore m v -> (
     match ee with
-    | EvictMerkle (EvictM k k') v' -> 
+    | EvictMerkle (EvictM k k') v' ->
       (* otherwise we would not have an eac failure *)
       assert(DVal? v && v' <> v);
 
@@ -491,28 +470,28 @@ let lemma_non_eac_instore_evictm (#p:pos)
       let i = max_eac_prefix tsle in
       let (e,tid) = index itsl i in
 
-      let itsli = prefix itsl i in  
+      let itsli = prefix itsl i in
       (* verifier thread state of tid after itsli *)
       let vsi = verifier_thread_state itsli tid in
 
       let itsli' = prefix itsl (i + 1) in
-      let vsi' = verifier_thread_state itsli' tid in    
-      lemma_verifier_thread_state_extend itsli';  
-      assert(vsi' == t_verify_step vsi e);    
+      let vsi' = verifier_thread_state itsli' tid in
+      lemma_verifier_thread_state_extend itsli';
+      assert(vsi' == t_verify_step vsi e);
 
       (* the thread store of tid contains k *)
       assert(store_contains (thread_store vsi) k);
 
-      lemma_ext_evict_val_is_stored_val itsl i;      
+      lemma_ext_evict_val_is_stored_val itsl i;
       assert(v' = stored_value (thread_store vsi) k);
 
       (* the tid of the last add to k prior to i *)
-      let ltid = last_add_tid itsli k in      
+      let ltid = last_add_tid itsli k in
 
       (* the store of ltid contains k and the value is v *)
-      lemma_eac_state_instore itsli k;      
+      lemma_eac_state_instore itsli k;
       assert(v = stored_value (thread_store (verifier_thread_state itsli ltid)) k);
-      
+
       if ltid = tid then
         (* since both v' and v are equal to stored value, v = v' => a contradiction *)
         hash_collision_contra()
@@ -525,33 +504,33 @@ let lemma_non_eac_instore_evictm (#p:pos)
       )
     )
 
-let lemma_non_eac_instore_evictb (#p:pos)   
+let lemma_non_eac_instore_evictb (#p:pos)
   (itsl: non_eac_ts_log p{
     EACInStore? (last_valid_eac_state itsl)  /\
     EvictB? (to_vlog_entry (invalidating_log_entry itsl))
    })
-  : hash_collision_gen = 
-  let st = last_valid_eac_state itsl in   
+  : hash_collision_gen =
+  let st = last_valid_eac_state itsl in
   let ee = invalidating_log_entry itsl in
   assert(eac_add ee st = EACFail);
   match st with
   | EACInStore m v -> (
     match ee with
-    | EvictBlum (EvictB k t) v' tid' ->     
-      assert(DVal? v && v' <> v || m <> BAdd);          
+    | EvictBlum (EvictB k t) v' tid' ->
+      assert(DVal? v && v' <> v || m <> BAdd);
 
       let tsle = time_seq_ext itsl in
       let i = max_eac_prefix tsle in
       let (e,tid) = index itsl i in
 
-      let itsli = prefix itsl i in  
+      let itsli = prefix itsl i in
       (* verifier thread state of tid after itsli *)
       let vsi = verifier_thread_state itsli tid in
 
       let itsli' = prefix itsl (i + 1) in
-      let vsi' = verifier_thread_state itsli' tid in    
-      lemma_verifier_thread_state_extend itsli';  
-      assert(vsi' == t_verify_step vsi e);    
+      let vsi' = verifier_thread_state itsli' tid in
+      lemma_verifier_thread_state_extend itsli';
+      assert(vsi' == t_verify_step vsi e);
 
       (* the thread store of tid contains k *)
       assert(store_contains (thread_store vsi) k);
@@ -571,7 +550,7 @@ let lemma_non_eac_instore_evictb (#p:pos)
         lemma_eac_state_instore itsli k;
         assert(stored_value (thread_store vsi) k = v);
 
-        lemma_ext_evict_val_is_stored_val itsl i;      
+        lemma_ext_evict_val_is_stored_val itsl i;
         assert(v' = stored_value (thread_store vsi) k);
 
         hash_collision_contra()
@@ -586,33 +565,33 @@ let lemma_non_eac_instore_evictb (#p:pos)
       )
   )
 
-let lemma_non_eac_instore_evictbm (#p:pos)   
+let lemma_non_eac_instore_evictbm (#p:pos)
   (itsl: non_eac_ts_log p{
     EACInStore? (last_valid_eac_state itsl)  /\
     EvictBM? (to_vlog_entry (invalidating_log_entry itsl))
    })
-  : hash_collision_gen = 
-  let st = last_valid_eac_state itsl in   
+  : hash_collision_gen =
+  let st = last_valid_eac_state itsl in
   let ee = invalidating_log_entry itsl in
   assert(eac_add ee st = EACFail);
   match st with
   | EACInStore m v -> (
     match ee with
-    | EvictBlum (EvictBM k k' t) v' tid' ->     
-      assert(DVal? v && v' <> v || m <> MAdd);        
+    | EvictBlum (EvictBM k k' t) v' tid' ->
+      assert(DVal? v && v' <> v || m <> MAdd);
       let tsle = time_seq_ext itsl in
       let i = max_eac_prefix tsle in
       let (e,tid) = index itsl i in
 
-      let itsli = prefix itsl i in  
+      let itsli = prefix itsl i in
       (* verifier thread state of tid after itsli *)
       let vsi = verifier_thread_state itsli tid in
 
       let itsli' = prefix itsl (i + 1) in
-      let vsi' = verifier_thread_state itsli' tid in    
-      lemma_verifier_thread_state_extend itsli';  
-      assert(vsi' == t_verify_step vsi e);    
-      
+      let vsi' = verifier_thread_state itsli' tid in
+      lemma_verifier_thread_state_extend itsli';
+      assert(vsi' == t_verify_step vsi e);
+
       (* the thread store of tid contains k *)
       assert(store_contains (thread_store vsi) k);
 
@@ -631,12 +610,12 @@ let lemma_non_eac_instore_evictbm (#p:pos)
         lemma_eac_state_instore itsli k;
         assert(stored_value (thread_store vsi) k = v);
 
-        lemma_ext_evict_val_is_stored_val itsl i;      
+        lemma_ext_evict_val_is_stored_val itsl i;
         assert(v' = stored_value (thread_store vsi) k);
 
         hash_collision_contra()
       )
-      else (    
+      else (
         (* only the store of last add contains the key k *)
         lemma_eac_state_instore2 itsli k tid;
         assert(not (store_contains (thread_store vsi) k));
@@ -647,42 +626,42 @@ let lemma_non_eac_instore_evictbm (#p:pos)
  )
 
 
-let lemma_non_eac_evicted_requires_key_in_store (#p:pos)   
+let lemma_non_eac_evicted_requires_key_in_store (#p:pos)
   (itsl: non_eac_ts_log p{
     EC.is_eac_state_evicted (last_valid_eac_state itsl)  /\
     requires_key_in_store (to_vlog_entry (invalidating_log_entry itsl))
    })
-  : hash_collision_gen = 
-  let st = last_valid_eac_state itsl in   
+  : hash_collision_gen =
+  let st = last_valid_eac_state itsl in
   let ee = invalidating_log_entry itsl in
-  assert(eac_add ee st = EACFail);  
+  assert(eac_add ee st = EACFail);
 
   let tsle = time_seq_ext itsl in
   let i = max_eac_prefix tsle in
   let (e,tid) = index itsl i in
   let k = V.key_of e in
-  let itsli = prefix itsl i in  
+  let itsli = prefix itsl i in
   (* verifier thread state of tid after itsli *)
   let vsi = verifier_thread_state itsli tid in
 
   let itsli' = prefix itsl (i + 1) in
-  let vsi' = verifier_thread_state itsli' tid in    
-  lemma_verifier_thread_state_extend itsli';  
-  assert(vsi' == t_verify_step vsi e);    
-  
+  let vsi' = verifier_thread_state itsli' tid in
+  lemma_verifier_thread_state_extend itsli';
+  assert(vsi' == t_verify_step vsi e);
+
   assert(store_contains (thread_store vsi) k);
   lemma_eac_state_evicted_store itsli k tid;
   hash_collision_contra()
 
-let lemma_non_eac_evicted_merkle_addm (#p:pos)   
+let lemma_non_eac_evicted_merkle_addm (#p:pos)
   (itsl: non_eac_ts_log p{
     EACEvictedMerkle? (last_valid_eac_state itsl)  /\
     AddM? (to_vlog_entry (invalidating_log_entry itsl))
    })
-  : hash_collision_gen = 
-  let st = last_valid_eac_state itsl in   
+  : hash_collision_gen =
+  let st = last_valid_eac_state itsl in
   let ee = invalidating_log_entry itsl in
-  assert(eac_add ee st = EACFail);  
+  assert(eac_add ee st = EACFail);
   match st with
   | EACEvictedMerkle v_e -> (
     match ee with
@@ -692,14 +671,14 @@ let lemma_non_eac_evicted_merkle_addm (#p:pos)
       let i = max_eac_prefix tsle in
       let (e,tid) = index itsl i in
 
-      let itsli = prefix itsl i in  
+      let itsli = prefix itsl i in
       (* verifier thread state of tid after itsli *)
       let vsi = verifier_thread_state itsli tid in
 
       let itsli' = prefix itsl (i + 1) in
-      let vsi' = verifier_thread_state itsli' tid in    
-      lemma_verifier_thread_state_extend itsli';  
-      assert(vsi' == t_verify_step vsi e);    
+      let vsi' = verifier_thread_state itsli' tid in
+      lemma_verifier_thread_state_extend itsli';
+      assert(vsi' == t_verify_step vsi e);
 
       (* k' is a proper ancestor, so k cannot be root *)
       assert(k <> Root);
@@ -725,18 +704,18 @@ let lemma_non_eac_evicted_merkle_addm (#p:pos)
       assert(Desc?.h dh = hashfn v_e);
 
       (* which gives us a hash collision *)
-      SingleHashCollision (Collision v v_e)     
+      SingleHashCollision (Collision v v_e)
     )
 
-let lemma_non_eac_evicted_blum_addm (#p:pos)   
+let lemma_non_eac_evicted_blum_addm (#p:pos)
   (itsl: non_eac_ts_log p{
     EACEvictedBlum? (last_valid_eac_state itsl)  /\
     AddM? (to_vlog_entry (invalidating_log_entry itsl))
    })
-  : hash_collision_gen = 
-  let st = last_valid_eac_state itsl in   
+  : hash_collision_gen =
+  let st = last_valid_eac_state itsl in
   let ee = invalidating_log_entry itsl in
-  assert(eac_add ee st = EACFail);  
+  assert(eac_add ee st = EACFail);
   match st with
   | EACEvictedBlum v_e _ _ -> (
     match ee with
@@ -745,14 +724,14 @@ let lemma_non_eac_evicted_blum_addm (#p:pos)
       let i = max_eac_prefix tsle in
       let (e,tid) = index itsl i in
 
-      let itsli = prefix itsl i in  
+      let itsli = prefix itsl i in
       (* verifier thread state of tid after itsli *)
       let vsi = verifier_thread_state itsli tid in
 
       let itsli' = prefix itsl (i + 1) in
-      let vsi' = verifier_thread_state itsli' tid in    
-      lemma_verifier_thread_state_extend itsli';  
-      assert(vsi' == t_verify_step vsi e);    
+      let vsi' = verifier_thread_state itsli' tid in
+      lemma_verifier_thread_state_extend itsli';
+      assert(vsi' == t_verify_step vsi e);
 
       (* k' is a proper ancestor, so k cannot be root *)
       assert(k <> Root);
@@ -763,32 +742,32 @@ let lemma_non_eac_evicted_blum_addm (#p:pos)
 
       (* k' points to k *)
       lemma_proving_ancestor_points_to_self itsli k;
-      lemma_eac_value_is_stored_value itsli k' tid;      
+      lemma_eac_value_is_stored_value itsli k' tid;
       let mv' = to_merkle_value (stored_value (thread_store vsi) k') in
       let d = desc_dir k k' in
       let dh = desc_hash_dir mv' d in
       assert(Desc?.k dh = k);
       assert(Desc?.b dh = false);
-      
+
       (* since m = BAdd, this bit should be set to true, a contradiction *)
       lemma_proving_ancestor_blum_bit itsli k;
-      hash_collision_contra()      
+      hash_collision_contra()
   )
 
-let lemma_non_eac_evicted_merkle_addb (#p:pos)   
+let lemma_non_eac_evicted_merkle_addb (#p:pos)
   (itsl: non_eac_ts_log p{
-    VG.hash_verifiable (partition_idx_seq itsl) /\  
+    VG.hash_verifiable (partition_idx_seq itsl) /\
     EACEvictedMerkle? (last_valid_eac_state itsl)  /\
     AddB? (to_vlog_entry (invalidating_log_entry itsl))
    })
-  : hash_collision_gen = 
-  (* hash verifiable - evict hash and add hash equal *)                          
-  let gl = partition_idx_seq itsl in                           
+  : hash_collision_gen =
+  (* hash verifiable - evict hash and add hash equal *)
+  let gl = partition_idx_seq itsl in
   assert(VG.hadd gl = VG.hevict gl);
-  
-  let st = last_valid_eac_state itsl in   
+
+  let st = last_valid_eac_state itsl in
   let ee = invalidating_log_entry itsl in
-  assert(eac_add ee st = EACFail);  
+  assert(eac_add ee st = EACFail);
   match st with
   | EACEvictedMerkle v_e -> (
     match ee with
@@ -797,14 +776,14 @@ let lemma_non_eac_evicted_merkle_addb (#p:pos)
       let i = max_eac_prefix tsle in
       let (e,tid) = index itsl i in
 
-      let itsli = prefix itsl i in  
+      let itsli = prefix itsl i in
       (* verifier thread state of tid after itsli *)
       let vsi = verifier_thread_state itsli tid in
 
       let itsli' = prefix itsl (i + 1) in
-      let vsi' = verifier_thread_state itsli' tid in    
-      lemma_verifier_thread_state_extend itsli';  
-      assert(vsi' == t_verify_step vsi e);    
+      let vsi' = verifier_thread_state itsli' tid in
+      lemma_verifier_thread_state_extend itsli';
+      assert(vsi' == t_verify_step vsi e);
 
       (* number of blum evicts is the same as blum adds in the first i entries *)
       lemma_evict_add_count_same_evictedm itsli k;
@@ -821,18 +800,18 @@ let lemma_non_eac_evicted_merkle_addb (#p:pos)
       lemma_ts_evict_set_key_extend2 itsli';
       assert(ts_evict_set_key itsli' k == ts_evict_set_key itsli k);
 
-      (* this implies that the size of the add set after processing (i+1) elements 
+      (* this implies that the size of the add set after processing (i+1) elements
          * is one larger than the evict set at this point *)
       assert(MS.size (ts_add_set_key itsli' k) = 1 + (MS.size (ts_evict_set_key itsli' k)));
 
-      (* this implies that in the first (i+1) entries there is an element whose membership in 
+      (* this implies that in the first (i+1) entries there is an element whose membership in
          * add multiset is > its membership in evict multiset *)
       let be = diff_elem (ts_add_set_key itsli' k) (ts_evict_set_key itsli' k) in
       lemma_ts_add_set_key_contains_only itsli' k be;
       assert(MH.key_of be = k);
 
       lemma_mem_key_add_set_same itsli' be;
-      lemma_mem_key_evict_set_same itsli' be;  
+      lemma_mem_key_evict_set_same itsli' be;
       assert(MS.mem be (ts_add_set itsli') > MS.mem be (ts_evict_set itsli'));
 
       (* the index of be in the add set *)
@@ -851,7 +830,7 @@ let lemma_non_eac_evicted_merkle_addb (#p:pos)
 
       (* this implies the membership of be in (overall) addset > membership in evict set *)
       (* so these two sets are not equal providing a hash collision *)
-      assert(MS.mem be (ts_add_set itsl) > MS.mem be (ts_evict_set itsl));  
+      assert(MS.mem be (ts_add_set itsl) > MS.mem be (ts_evict_set itsl));
 
       MS.lemma_not_equal (ts_add_set itsl) (ts_evict_set itsl) be;
       assert(~( (ts_add_set itsl) == (ts_evict_set itsl)));
@@ -866,17 +845,17 @@ let lemma_non_eac_evicted_merkle_addb (#p:pos)
       MultiHashCollision (MSCollision (g_add_seq gl) (g_evict_seq gl))
   )
 
-let lemma_non_eac_evicted_blum_addb (#p:pos)   
+let lemma_non_eac_evicted_blum_addb (#p:pos)
   (itsl: non_eac_ts_log p{
-    VG.hash_verifiable (partition_idx_seq itsl) /\  
+    VG.hash_verifiable (partition_idx_seq itsl) /\
     EACEvictedBlum? (last_valid_eac_state itsl)  /\
     AddB? (to_vlog_entry (invalidating_log_entry itsl))
    })
-  : hash_collision_gen = 
-  (* hash verifiable - evict hash and add hash equal *)                          
-  let gl = partition_idx_seq itsl in                           
+  : hash_collision_gen =
+  (* hash verifiable - evict hash and add hash equal *)
+  let gl = partition_idx_seq itsl in
 
-  let st = last_valid_eac_state itsl in   
+  let st = last_valid_eac_state itsl in
   let ee = invalidating_log_entry itsl in
   match st with
   | EACEvictedBlum v_e t j -> (
@@ -888,14 +867,14 @@ let lemma_non_eac_evicted_blum_addb (#p:pos)
     let i = max_eac_prefix tsle in
     let (e,tid) = index itsl i in
 
-    let itsli = prefix itsl i in  
+    let itsli = prefix itsl i in
     (* verifier thread state of tid after itsli *)
     let vsi = verifier_thread_state itsli tid in
 
     let itsli' = prefix itsl (i + 1) in
-    let vsi' = verifier_thread_state itsli' tid in    
-    lemma_verifier_thread_state_extend itsli';  
-    //assert(vsi' == t_verify_step vsi e);    
+    let vsi' = verifier_thread_state itsli' tid in
+    lemma_verifier_thread_state_extend itsli';
+    //assert(vsi' == t_verify_step vsi e);
 
     let be = blum_add_elem (index itsl i) in
 
@@ -904,7 +883,7 @@ let lemma_non_eac_evicted_blum_addb (#p:pos)
     let i' = last_idx_of_key itsli k in
     //assert(is_blum_evict (index itsli i'));
 
-    (* since EAC failed, the blum element added to evict set at i' <> blum element added to 
+    (* since EAC failed, the blum element added to evict set at i' <> blum element added to
      * add set at i *)
     let be' = blum_evict_elem itsli i' in
     //assert(be <> be');
@@ -919,7 +898,7 @@ let lemma_non_eac_evicted_blum_addb (#p:pos)
       (* from clock ordering j has to occur before i *)
       lemma_evict_before_add3 itsl i j;
       //assert (j < i);
-      
+
       //assert(entry_of_key k (index itsli j));
       lemma_last_index_correct2 (entry_of_key k) itsli j;
 
@@ -948,43 +927,44 @@ let lemma_non_eac_evicted_blum_addb (#p:pos)
       lemma_ghevict_correct gl;
       lemma_g_hadd_correct gl;
 
-      MultiHashCollision (MSCollision (g_add_seq gl) (g_evict_seq gl))      
+      MultiHashCollision (MSCollision (g_add_seq gl) (g_evict_seq gl))
     )
     else (
-      
+
       lemma_ts_add_set_contains_add_elem itsl i;
       //assert(MS.contains be (ts_add_set itsl));
 
-      MS.lemma_not_equal (ts_add_set itsl) (ts_evict_set itsl) be;     
+      MS.lemma_not_equal (ts_add_set itsl) (ts_evict_set itsl) be;
       lemma_ts_evict_set_correct itsl;
-      lemma_ts_add_set_correct itsl;     
+      lemma_ts_add_set_correct itsl;
       //assert(~ (g_add_set gl == g_evict_set gl));
 
       lemma_ghevict_correct gl;
       lemma_g_hadd_correct gl;
 
-      MultiHashCollision (MSCollision (g_add_seq gl) (g_evict_seq gl))      
+      MultiHashCollision (MSCollision (g_add_seq gl) (g_evict_seq gl))
     )
  )
 *)
 
 
 
-let lemma_non_eac_time_seq_implies_hash_collision 
-  (itsl: neac_log {VG.hash_verifiable (g_vlog_of itsl)}): hash_collision_gen =   
+let lemma_non_eac_time_seq_implies_hash_collision
+  (itsl: neac_log {VG.hash_verifiable (g_vlog_of itsl)}): hash_collision_gen =
   let i = TL.eac_boundary itsl in
   let st = TL.eac_state_pre itsl i in
-  let ee:vlog_entry_ext = TL.vlog_entry_ext_at itsl i in 
-  
+  let ee:vlog_entry_ext = TL.vlog_entry_ext_at itsl i in
+
   match st with
   | EACInit -> (
-      match ee with 
+      match ee with
       | NEvict (Get _ _) -> lemma_non_eac_init_requires_key_in_store itsl
       | NEvict (Put _ _) -> lemma_non_eac_init_requires_key_in_store itsl
+      | NEvict (AddB _ _ _) -> lemma_non_eac_init_addb itsl
+      | NEvict (AddM (k,v) _) -> lemma_non_eac_init_addm itsl
       | EvictMerkle (EvictM _ _) _ -> lemma_non_eac_init_evict itsl
       | EvictBlum (EvictB _ _) _ _ -> lemma_non_eac_init_evict itsl
-      | EvictBlum (EvictBM _ _ _) _ _ -> lemma_non_eac_init_evict itsl      
-      | _ -> admit()
+      | EvictBlum (EvictBM _ _ _) _ _ -> lemma_non_eac_init_evict itsl
     )
   | _ ->
 
@@ -995,16 +975,16 @@ let lemma_non_eac_time_seq_implies_hash_collision
 
   last_valid_eac_state itsl = EACInit /\
                            VT.requires_key_in_store (to_vlog_entry (invalidating_log_entry itsl)) /\
-                           Root <> V.key_of (to_vlog_entry (invalidating_log_entry itsl))}):  
-                           
+                           Root <> V.key_of (to_vlog_entry (invalidating_log_entry itsl))}):
+
   let st = last_valid_eac_state itsl in
   let ee = invalidating_log_entry itsl in
-  let tsle = time_seq_ext itsl in  
+  let tsle = time_seq_ext itsl in
   let i = max_eac_prefix tsle in
-  
+
   match st with
   | EACInit -> (
-      match ee with 
+      match ee with
       | NEvict (Get _ _) -> lemma_non_eac_init_requires_key_in_store itsl
       | NEvict (Put _ _) -> lemma_non_eac_init_requires_key_in_store itsl
       | NEvict (AddB _ _ _) -> lemma_non_eac_init_addb itsl
@@ -1014,7 +994,7 @@ let lemma_non_eac_time_seq_implies_hash_collision
       | EvictBlum (EvictBM _ _ _) _ _ -> lemma_non_eac_init_evict itsl
     )
   | EACInStore m v -> (
-    match ee with 
+    match ee with
       | NEvict (Get _ _) -> lemma_non_eac_instore_get itsl
       | NEvict (Put _ _) -> lemma_non_eac_instore_put itsl
       | NEvict (AddB _ _ _) -> lemma_non_eac_instore_addb itsl
@@ -1024,7 +1004,7 @@ let lemma_non_eac_time_seq_implies_hash_collision
       | EvictBlum (EvictBM _ _ _) _ _ -> lemma_non_eac_instore_evictbm itsl
   )
   | EACEvictedMerkle v -> (
-    match ee with 
+    match ee with
       | NEvict (Get _ _) -> lemma_non_eac_evicted_requires_key_in_store itsl
       | NEvict (Put _ _) -> lemma_non_eac_evicted_requires_key_in_store itsl
       | NEvict (AddB _ _ _) ->  lemma_non_eac_evicted_merkle_addb itsl
@@ -1034,7 +1014,7 @@ let lemma_non_eac_time_seq_implies_hash_collision
       | EvictBlum (EvictBM _ _ _) _ _ -> lemma_non_eac_evicted_requires_key_in_store itsl
   )
   | EACEvictedBlum v t tid -> (
-    match ee with 
+    match ee with
       | NEvict (Get _ _) -> lemma_non_eac_evicted_requires_key_in_store itsl
       | NEvict (Put _ _) -> lemma_non_eac_evicted_requires_key_in_store itsl
       | NEvict (AddB _ _ _) ->  lemma_non_eac_evicted_blum_addb itsl
